a few simple props of the new PER

theories/Core/Semantic/WPER/Definitions.v
@@ -3,7 +3,7 @@ From Equations Require Import Equations.
 
 From Mctt Require Import LibTactics.
 From Mctt.Core Require Import Base.
-From Mctt.Core.Syntactic Require Import WeakCong.
+From Mctt.Core.Syntactic.WCong Require Import Definitions.
 From Mctt.Core.Semantic Require Export Domain Evaluation Readback.
 Import Domain_Notations.
 
@@ -95,26 +95,26 @@ Section Per_univ_elem_core_def.
           (lt_j_i : j < i),
           j = j' ->
           (elem_rel <~> per_univ_rec lt_j_i) ->
-          {{ DF 𝕌@j ≈ 𝕌@j' ∈ per_univ_elem_core ↘ elem_rel }} }
+          {{ DF 𝕌@j ≈≈ 𝕌@j' ∈ per_univ_elem_core ↘ elem_rel }} }
   | per_univ_elem_core_nat :
     forall (elem_rel : relation domain),
       (elem_rel <~> per_nat) ->
-      {{ DF ℕ ≈ ℕ ∈ per_univ_elem_core ↘ elem_rel }}
+      {{ DF ℕ ≈≈ ℕ ∈ per_univ_elem_core ↘ elem_rel }}
   | per_univ_elem_core_pi :
     `{ forall (in_rel : relation domain)
-         (out_rel : forall {c c'} (equiv_c_c' : {{ Dom c ≈ c' ∈ in_rel }}), relation domain)
+         (out_rel : forall {c c'} (equiv_c_c' : {{ Dom c ≈≈ c' ∈ in_rel }}), relation domain)
          (elem_rel : relation domain)
-         (equiv_a_a' : {{ DF a ≈ a' ∈ per_univ_elem_core ↘ in_rel}}),
+         (equiv_a_a' : {{ DF a ≈≈ a' ∈ per_univ_elem_core ↘ in_rel}}),
           PER in_rel ->
-          (forall {c c'} (equiv_c_c' : {{ Dom c ≈ c' ∈ in_rel }}),
+          (forall {c c'} (equiv_c_c' : {{ Dom c ≈≈ c' ∈ in_rel }}),
               rel_mod_eval per_univ_elem_core B d{{{ ρ ↦ c }}} B' d{{{ ρ' ↦ c' }}} (out_rel equiv_c_c')) ->
-          (elem_rel <~> fun f f' => forall c c' (equiv_c_c' : {{ Dom c ≈ c' ∈ in_rel }}), rel_mod_app f c f' c' (out_rel equiv_c_c')) ->
-          {{ DF Π a ρ B ≈ Π a' ρ' B' ∈ per_univ_elem_core ↘ elem_rel }} }
+          (elem_rel <~> fun f f' => forall c c' (equiv_c_c' : {{ Dom c ≈≈ c' ∈ in_rel }}), rel_mod_app f c f' c' (out_rel equiv_c_c')) ->
+          {{ DF Π a ρ B ≈≈ Π a' ρ' B' ∈ per_univ_elem_core ↘ elem_rel }} }
   | per_univ_elem_core_neut :
     `{ forall (elem_rel : relation domain),
-          {{ Dom b ≈ b' ∈ per_bot }} ->
+          {{ Dom b ≈≈ b' ∈ per_bot }} ->
           (elem_rel <~> per_ne) ->
-          {{ DF ⇑ a b ≈ ⇑ a' b' ∈ per_univ_elem_core ↘ elem_rel }} }
+          {{ DF ⇑ a b ≈≈ ⇑ a' b' ∈ per_univ_elem_core ↘ elem_rel }} }
   .
 
   Hypothesis
@@ -128,22 +128,22 @@ Section Per_univ_elem_core_def.
           motive elem_rel d{{{ ℕ }}} d{{{ ℕ }}})
       (case_Pi :
         forall {a ρ B a' ρ' B' in_rel}
-           (out_rel : forall {c c'} (equiv_c_c' : {{ Dom c ≈ c' ∈ in_rel }}), relation domain)
+           (out_rel : forall {c c'} (equiv_c_c' : {{ Dom c ≈≈ c' ∈ in_rel }}), relation domain)
            {elem_rel},
-          {{ DF a ≈ a' ∈ per_univ_elem_core ↘ in_rel }} ->
+          {{ DF a ≈≈ a' ∈ per_univ_elem_core ↘ in_rel }} ->
           motive in_rel a a' ->
           PER in_rel ->
-          (forall {c c'} (equiv_c_c' : {{ Dom c ≈ c' ∈ in_rel }}),
-              rel_mod_eval (fun R x y => {{ DF x ≈ y ∈ per_univ_elem_core ↘ R }} /\ motive R x y) B d{{{ ρ ↦ c }}} B' d{{{ ρ' ↦ c' }}} (out_rel equiv_c_c')) ->
-          (elem_rel <~> fun f f' => forall c c' (equiv_c_c' : {{ Dom c ≈ c' ∈ in_rel }}), rel_mod_app f c f' c' (out_rel equiv_c_c')) ->
+          (forall {c c'} (equiv_c_c' : {{ Dom c ≈≈ c' ∈ in_rel }}),
+              rel_mod_eval (fun R x y => {{ DF x ≈≈ y ∈ per_univ_elem_core ↘ R }} /\ motive R x y) B d{{{ ρ ↦ c }}} B' d{{{ ρ' ↦ c' }}} (out_rel equiv_c_c')) ->
+          (elem_rel <~> fun f f' => forall c c' (equiv_c_c' : {{ Dom c ≈≈ c' ∈ in_rel }}), rel_mod_app f c f' c' (out_rel equiv_c_c')) ->
           motive elem_rel d{{{ Π a ρ B }}} d{{{ Π a' ρ' B' }}})
       (case_ne : forall {a b a' b' elem_rel},
-          {{ Dom b ≈ b' ∈ per_bot }} ->
+          {{ Dom b ≈≈ b' ∈ per_bot }} ->
           (elem_rel <~> per_ne) ->
           motive elem_rel d{{{ ⇑ a b }}} d{{{ ⇑ a' b' }}}).
 
   #[derive(equations=no, eliminator=no)]
-  Equations per_univ_elem_core_strong_ind R a b (H : {{ DF a ≈ b ∈ per_univ_elem_core ↘ R }}) : {{ DF a ≈ b ∈ motive ↘ R }} :=
+  Equations per_univ_elem_core_strong_ind R a b (H : {{ DF a ≈≈ b ∈ per_univ_elem_core ↘ R }}) : {{ DF a ≈≈ b ∈ motive ↘ R }} :=
   | R, a, b, (per_univ_elem_core_univ _ lt_j_i HE eq)                 => case_U lt_j_i HE eq;
   | R, a, b, (per_univ_elem_core_nat _ HE)                            => case_nat HE;
   | R, a, b, (per_univ_elem_core_pi _ out_rel _ equiv_a_a' per HT HE) =>
@@ -161,9 +161,9 @@ End Per_univ_elem_core_def.
 Hint Constructors per_univ_elem_core : mctt.
 
 Equations per_univ_elem (i : nat) : relation domain -> domain -> domain -> Prop by wf i :=
-| i => per_univ_elem_core i (fun j lt_j_i a a' => exists R', {{ DF a ≈ a' ∈ per_univ_elem j ↘ R' }}).
+| i => per_univ_elem_core i (fun j lt_j_i a a' => exists R', {{ DF a ≈≈ a' ∈ per_univ_elem j ↘ R' }}).
 
-Definition per_univ (i : nat) : relation domain := fun a a' => exists R', {{ DF a ≈ a' ∈ per_univ_elem i ↘ R' }}.
+Definition per_univ (i : nat) : relation domain := fun a a' => exists R', {{ DF a ≈≈ a' ∈ per_univ_elem i ↘ R' }}.
 #[global]
 Arguments per_univ _ _ _ /.
 #[export]
@@ -174,7 +174,7 @@ Hint Unfold per_univ : mctt.
 Lemma per_univ_elem_core_univ' : forall j i elem_rel,
     j < i ->
     (elem_rel <~> per_univ j) ->
-    {{ DF 𝕌@j ≈ 𝕌@j ∈ per_univ_elem i ↘ elem_rel }}.
+    {{ DF 𝕌@j ≈≈ 𝕌@j ∈ per_univ_elem i ↘ elem_rel }}.
 Proof.
   intros.
   simp per_univ_elem.
@@ -192,24 +192,24 @@ Section Per_univ_elem_ind_def.
       (case_U : forall i {j j' elem_rel},
           j < i -> j = j' ->
           (elem_rel <~> per_univ j) ->
-          (forall A B R, {{ DF A ≈ B ∈ per_univ_elem j ↘ R }} -> motive j R A B) ->
+          (forall A B R, {{ DF A ≈≈ B ∈ per_univ_elem j ↘ R }} -> motive j R A B) ->
           motive i elem_rel d{{{ 𝕌@j }}} d{{{ 𝕌@j' }}})
       (case_N : forall i {elem_rel},
           (elem_rel <~> per_nat) ->
           motive i elem_rel d{{{ ℕ }}} d{{{ ℕ }}})
       (case_Pi :
         forall i {a ρ B a' ρ' B' in_rel}
-           (out_rel : forall {c c'} (equiv_c_c' : {{ Dom c ≈ c' ∈ in_rel }}), relation domain)
+           (out_rel : forall {c c'} (equiv_c_c' : {{ Dom c ≈≈ c' ∈ in_rel }}), relation domain)
            {elem_rel},
-          {{ DF a ≈ a' ∈ per_univ_elem i ↘ in_rel }} ->
+          {{ DF a ≈≈ a' ∈ per_univ_elem i ↘ in_rel }} ->
           motive i in_rel a a' ->
           PER in_rel ->
-          (forall {c c'} (equiv_c_c' : {{ Dom c ≈ c' ∈ in_rel }}),
-              rel_mod_eval (fun R x y => {{ DF x ≈ y ∈ per_univ_elem i ↘ R }} /\ motive i R x y) B d{{{ ρ ↦ c }}} B' d{{{ ρ' ↦ c' }}} (out_rel equiv_c_c')) ->
-          (elem_rel <~> fun f f' => forall c c' (equiv_c_c' : {{ Dom c ≈ c' ∈ in_rel }}), rel_mod_app f c f' c' (out_rel equiv_c_c')) ->
+          (forall {c c'} (equiv_c_c' : {{ Dom c ≈≈ c' ∈ in_rel }}),
+              rel_mod_eval (fun R x y => {{ DF x ≈≈ y ∈ per_univ_elem i ↘ R }} /\ motive i R x y) B d{{{ ρ ↦ c }}} B' d{{{ ρ' ↦ c' }}} (out_rel equiv_c_c')) ->
+          (elem_rel <~> fun f f' => forall c c' (equiv_c_c' : {{ Dom c ≈≈ c' ∈ in_rel }}), rel_mod_app f c f' c' (out_rel equiv_c_c')) ->
           motive i elem_rel d{{{ Π a ρ B }}} d{{{ Π a' ρ' B' }}})
       (case_ne : forall i {a b a' b' elem_rel},
-          {{ Dom b ≈ b' ∈ per_bot }} ->
+          {{ Dom b ≈≈ b' ∈ per_bot }} ->
           (elem_rel <~> per_ne) ->
           motive i elem_rel d{{{ ⇑ a b }}} d{{{ ⇑ a' b' }}}).
 
@@ -218,7 +218,7 @@ Section Per_univ_elem_ind_def.
 
   #[derive(equations=no, eliminator=no), tactic="def_simp"]
   Equations per_univ_elem_ind' (i : nat) (R : relation domain) (a b : domain)
-    (H : {{ DF a ≈ b ∈ per_univ_elem_core i (fun j lt_j_i a a' => exists R', {{ DF a ≈ a' ∈ per_univ_elem j ↘ R' }}) ↘ R }}) : {{ DF a ≈ b ∈ motive i ↘ R }} by wf i :=
+    (H : {{ DF a ≈≈ b ∈ per_univ_elem_core i (fun j lt_j_i a a' => exists R', {{ DF a ≈≈ a' ∈ per_univ_elem j ↘ R' }}) ↘ R }}) : {{ DF a ≈≈ b ∈ motive i ↘ R }} by wf i :=
   | i, R, a, b, H =>
       per_univ_elem_core_strong_ind i _ (motive i)
         (fun _ _ _ j_lt_i eq HE => case_U i j_lt_i eq HE (fun A B R' H' => per_univ_elem_ind' _ R' A B _))
@@ -238,7 +238,7 @@ Reserved Notation "'Sub' a <: b 'at' i" (in custom judg at level 90, a custom do
 
 Inductive per_subtyp : nat -> domain -> domain -> Prop :=
 | per_subtyp_neut :
-  `( {{ Dom b ≈ b' ∈ per_bot }} ->
+  `( {{ Dom b ≈≈ b' ∈ per_bot }} ->
      {{ Sub ⇑ a b <: ⇑ a' b' at i }} )
 | per_subtyp_nat :
   `( {{ Sub ℕ <: ℕ at i }} )
@@ -249,14 +249,14 @@ Inductive per_subtyp : nat -> domain -> domain -> Prop :=
 | per_subtyp_pi :
   `( forall (in_rel : relation domain) elem_rel elem_rel',
         {{ Sub a' <: a at i }} ->
-        {{ DF a' ≈ a' ∈ per_univ_elem i ↘ in_rel }} ->
+        {{ DF a' ≈≈ a' ∈ per_univ_elem i ↘ in_rel }} ->
         (forall c c' b b',
-            {{ Dom c ≈ c' ∈ in_rel }} ->
+            {{ Dom c ≈≈ c' ∈ in_rel }} ->
             {{ ⟦ B ⟧ ρ ↦ c ↘ b }} ->
             {{ ⟦ B' ⟧ ρ' ↦ c' ↘ b' }} ->
             {{ Sub b <: b' at i }}) ->
-        {{ DF Π a ρ B ≈ Π a ρ B ∈ per_univ_elem i ↘ elem_rel }} ->
-        {{ DF Π a' ρ' B' ≈ Π a' ρ' B' ∈ per_univ_elem i ↘ elem_rel' }} ->
+        {{ DF Π a ρ B ≈≈ Π a ρ B ∈ per_univ_elem i ↘ elem_rel }} ->
+        {{ DF Π a' ρ' B' ≈≈ Π a' ρ' B' ∈ per_univ_elem i ↘ elem_rel' }} ->
         {{ Sub Π a ρ B <: Π a' ρ' B' at i }})
 where "'Sub' a <: b 'at' i" := (per_subtyp i a b) (in custom judg) : type_scope.
 
@@ -276,19 +276,19 @@ Inductive per_ctx_env : relation env -> ctx -> ctx -> Prop :=
 | per_ctx_env_nil :
   `{ forall env_rel,
         (env_rel <~> fun ρ ρ' => True) ->
-        {{ EF ⋅ ≈ ⋅ ∈ per_ctx_env ↘ env_rel }} }
+        {{ EF ⋅ ≈≈ ⋅ ∈ per_ctx_env ↘ env_rel }} }
 | per_ctx_env_cons :
   `{ forall tail_rel
-        (head_rel : forall {ρ ρ'} (equiv_ρ_ρ' : {{ Dom ρ ≈ ρ' ∈ tail_rel }}), relation domain)
+        (head_rel : forall {ρ ρ'} (equiv_ρ_ρ' : {{ Dom ρ ≈≈ ρ' ∈ tail_rel }}), relation domain)
         env_rel
-        (equiv_Γ_Γ' : {{ EF Γ ≈ Γ' ∈ per_ctx_env ↘ tail_rel }}),
+        (equiv_Γ_Γ' : {{ EF Γ ≈≈ Γ' ∈ per_ctx_env ↘ tail_rel }}),
         PER tail_rel ->
-        (forall {ρ ρ'} (equiv_ρ_ρ' : {{ Dom ρ ≈ ρ' ∈ tail_rel }}),
+        (forall {ρ ρ'} (equiv_ρ_ρ' : {{ Dom ρ ≈≈ ρ' ∈ tail_rel }}),
             rel_typ i A ρ A' ρ' (head_rel equiv_ρ_ρ')) ->
         (env_rel <~> fun ρ ρ' =>
-             exists (equiv_ρ_drop_ρ'_drop : {{ Dom ρ ↯ ≈ ρ' ↯ ∈ tail_rel }}),
-               {{ Dom ^(ρ 0) ≈ ^(ρ' 0) ∈ head_rel equiv_ρ_drop_ρ'_drop }}) ->
-        {{ EF Γ, A ≈ Γ', A' ∈ per_ctx_env ↘ env_rel }} }
+             exists (equiv_ρ_drop_ρ'_drop : {{ Dom ρ ↯ ≈≈ ρ' ↯ ∈ tail_rel }}),
+               {{ Dom ^(ρ 0) ≈≈ ^(ρ' 0) ∈ head_rel equiv_ρ_drop_ρ'_drop }}) ->
+        {{ EF Γ, A ≈≈ Γ', A' ∈ per_ctx_env ↘ env_rel }} }
 .
 #[export]
 Hint Constructors per_ctx_env : mctt.
@@ -310,14 +310,14 @@ Inductive per_ctx_subtyp : ctx -> ctx -> Prop :=
 | per_ctx_subtyp_cons :
   `{ forall tail_rel env_rel env_rel',
         {{ SubE Γ <: Γ' }} ->
-        {{ EF Γ ≈ Γ ∈ per_ctx_env ↘ tail_rel }} ->
+        {{ EF Γ ≈≈ Γ ∈ per_ctx_env ↘ tail_rel }} ->
         (forall ρ ρ' a a'
-           (equiv_ρ_ρ' : {{ Dom ρ ≈ ρ' ∈ tail_rel }}),
+           (equiv_ρ_ρ' : {{ Dom ρ ≈≈ ρ' ∈ tail_rel }}),
             {{ ⟦ A ⟧ ρ ↘ a }} ->
             {{ ⟦ A' ⟧ ρ' ↘ a' }} ->
             {{ Sub a <: a' at i }}) ->
-        {{ EF Γ , A ≈ Γ , A ∈ per_ctx_env ↘ env_rel }} ->
-        {{ EF Γ' , A' ≈ Γ' , A' ∈ per_ctx_env ↘ env_rel' }} ->
+        {{ EF Γ , A ≈≈ Γ , A ∈ per_ctx_env ↘ env_rel }} ->
+        {{ EF Γ' , A' ≈≈ Γ' , A' ∈ per_ctx_env ↘ env_rel' }} ->
         {{ SubE Γ, A <: Γ', A' }} }
 where "'SubE' Γ <: Δ" := (per_ctx_subtyp Γ Δ) (in custom judg) : type_scope.
 
